feat: use Imperative_HOL

src/gen/Heap.hs
@@ -1,0 +1,37 @@
+{-# LANGUAGE EmptyDataDecls, RankNTypes, ScopedTypeVariables #-}
+
+module Heap where {
+
+import qualified Control.Monad;
+import qualified Control.Monad.ST;
+import qualified Data.STRef;
+import qualified Data.Array.ST;
+
+type RealWorld = Control.Monad.ST.RealWorld;
+type ST s a = Control.Monad.ST.ST s a;
+type STRef s a = Data.STRef.STRef s a;
+type STArray s a = Data.Array.ST.STArray s Integer a;
+
+newSTRef = Data.STRef.newSTRef;
+readSTRef = Data.STRef.readSTRef;
+writeSTRef = Data.STRef.writeSTRef;
+
+newArray :: Integer -> a -> ST s (STArray s a);
+newArray k = Data.Array.ST.newArray (0, k - 1);
+
+newListArray :: [a] -> ST s (STArray s a);
+newListArray xs = Data.Array.ST.newListArray (0, (fromInteger . toInteger . length) xs - 1) xs;
+
+newFunArray :: Integer -> (Integer -> a) -> ST s (STArray s a);
+newFunArray k f = Data.Array.ST.newListArray (0, k - 1) (map f [0..k-1]);
+
+lengthArray :: STArray s a -> ST s Integer;
+lengthArray a = Control.Monad.liftM (\(_, l) -> l + 1) (Data.Array.ST.getBounds a);
+
+readArray :: STArray s a -> Integer -> ST s a;
+readArray = Data.Array.ST.readArray;
+
+writeArray :: STArray s a -> Integer -> a -> ST s ();
+writeArray = Data.Array.ST.writeArray;
+
+}
