src/IOArray.thy
@@ -1,0 +1,41 @@
+theory IOArray
+  imports IO
+begin
+
+datatype 'a io_array = IOArray "'a ref" nat
+
+term "allocate"
+
+fun new_array :: "nat \<Rightarrow> 'a::heap io_array io" where
+  "new_array s = allocate s \<bind> (\<lambda>r. return (IOArray r s))"
+
+fun read_array :: "'a io_array \<Rightarrow> nat \<Rightarrow> 'a::heap io" where
+  "read_array (IOArray arr _) i = lookup (Ref (addr_of_ref arr + i))"
+
+fun write_array :: "'a io_array \<Rightarrow> nat \<Rightarrow> 'a::heap \<Rightarrow> unit io" where
+  "write_array (IOArray arr _) i val = update (Ref (addr_of_ref arr + i)) val"
+
+fun swap_array :: "'a::heap io_array \<Rightarrow> nat \<Rightarrow> nat \<Rightarrow> unit io" where
+  "swap_array arr i j = do {
+    valI \<leftarrow> read_array arr i;
+    valJ \<leftarrow> read_array arr j;
+    write_array arr j valI;
+    write_array arr i valJ;
+    return ()
+  }"
+
+(* IO Operations *)
+fun write_list_as_array :: "'a::heap list \<Rightarrow> 'a io_array io" where
+  "write_list_as_array xs = (do {
+    arr \<leftarrow> new_array (size xs);
+    forMu (enumerate 0 xs) (\<lambda>(i,x). write_array arr i x);
+    return arr
+  })"
+
+fun read_list_from_array :: "'a::heap io_array \<Rightarrow> 'a list io" where
+  "read_list_from_array (IOArray arr n) = mapM (\<lambda>i. read_array (IOArray arr n) i) (map nat [0..int n])"
+
+lemma list_write_read_id: "write_list_as_array xs \<bind> (\<lambda>arr. read_list_from_array arr) = return xs"
+  sorry
+
+end
